Primops: more modularization

src/typechecker/FStar.TypeChecker.Primops.Base.fst
@@ -36,22 +36,23 @@ let as_primitive_step_nbecbs is_strong (l, arity, u_arity, f, f_nbe) : primitive
     interpretation_nbe=(fun cb univs args -> f_nbe cb univs args)
 }
 
-let mk1 #a #r
-  (u_arity : int)
-  (name : Ident.lid)
-  {| EMB.embedding a |} {| NBE.embedding a |}
-  {| EMB.embedding r |} {| NBE.embedding r |}
+let mk_interp1 #a #r
+  {| EMB.embedding a |}
+  {| EMB.embedding r |}
   (f : a -> r)
-  : primitive_step =
-  let interp : interp_t =
+  : interp_t =
     fun psc cb us args ->
       match args with
       | [(a, _)] ->
         let! a = try_unembed_simple a in
         return (embed_simple psc.psc_range (f a))
       | _ -> None
-  in
-  let nbe_interp : nbe_interp_t =
+
+let mk_nbe_interp1 #a #r
+  {| NBE.embedding a |}
+  {| NBE.embedding r |}
+  (f : a -> r)
+  : nbe_interp_t =
     fun cbs us args ->
       match args with
       | [(a, _)] ->
@@ -59,7 +60,136 @@ let mk1 #a #r
         return (NBE.embed solve cbs r)
       | _ ->
         None
-  in
+
+let mk_interp2 #a #b #r
+  {| EMB.embedding a |}
+  {| EMB.embedding b |}
+  {| EMB.embedding r |}
+  (f : a -> b -> r)
+  : interp_t =
+    fun psc cb us args ->
+      match args with
+      | [(a, _); (b, _)] ->
+        let! r = f <$> try_unembed_simple a <*> try_unembed_simple b in
+        return (embed_simple psc.psc_range r)
+      | _ -> None
+
+let mk_nbe_interp2 #a #b #r
+  {| NBE.embedding a |}
+  {| NBE.embedding b |}
+  {| NBE.embedding r |}
+  (f : a -> b -> r)
+  : nbe_interp_t =
+    fun cbs us args ->
+      match args with
+      | [(a, _); (b, _)] ->
+        let! r = f <$> NBE.unembed solve cbs a <*> NBE.unembed solve cbs b in
+        return (NBE.embed solve cbs r)
+      | _ ->
+        None
+
+let mk_interp3 #a #b #c #r
+  {| EMB.embedding a |}
+  {| EMB.embedding b |}
+  {| EMB.embedding c |}
+  {| EMB.embedding r |}
+  (f : a -> b -> c -> r)
+  : interp_t =
+    fun psc cb us args ->
+      match args with
+      | [(a, _); (b, _); (c, _)] ->
+        let! r = f <$> try_unembed_simple a <*> try_unembed_simple b <*> try_unembed_simple c in
+        return (embed_simple psc.psc_range r)
+      | _ -> None
+
+let mk_nbe_interp3 #a #b #c #r
+  {| NBE.embedding a |}
+  {| NBE.embedding b |}
+  {| NBE.embedding c |}
+  {| NBE.embedding r |}
+  (f : a -> b -> c -> r)
+  : nbe_interp_t =
+    fun cbs us args ->
+      match args with
+      | [(a, _); (b, _); (c, _)] ->
+        let! r = f <$> NBE.unembed solve cbs a <*> NBE.unembed solve cbs b <*> NBE.unembed solve cbs c in
+        return (NBE.embed solve cbs r)
+      | _ ->
+        None
+
+let mk_interp4 #a #b #c #d #r
+  {| EMB.embedding a |}
+  {| EMB.embedding b |}
+  {| EMB.embedding c |}
+  {| EMB.embedding d |}
+  {| EMB.embedding r |}
+  (f : a -> b -> c -> d -> r)
+  : interp_t =
+    fun psc cb us args ->
+      match args with
+      | [(a, _); (b, _); (c, _); (d, _)] ->
+        let! r = f <$> try_unembed_simple a <*> try_unembed_simple b <*> try_unembed_simple c <*> try_unembed_simple d in
+        return (embed_simple psc.psc_range r)
+      | _ -> None
+
+let mk_nbe_interp4 #a #b #c #d #r
+  {| NBE.embedding a |}
+  {| NBE.embedding b |}
+  {| NBE.embedding c |}
+  {| NBE.embedding d |}
+  {| NBE.embedding r |}
+  (f : a -> b -> c -> d -> r)
+  : nbe_interp_t =
+    fun cbs us args ->
+      match args with
+      | [(a, _); (b, _); (c, _); (d, _)] ->
+        let! r = f <$> NBE.unembed solve cbs a <*> NBE.unembed solve cbs b <*> NBE.unembed solve cbs c <*> NBE.unembed solve cbs d in
+        return (NBE.embed solve cbs r)
+      | _ ->
+        None
+
+let mk_interp5 #a #b #c #d #e #r
+  {| EMB.embedding a |}
+  {| EMB.embedding b |}
+  {| EMB.embedding c |}
+  {| EMB.embedding d |}
+  {| EMB.embedding e |}
+  {| EMB.embedding r |}
+  (f : a -> b -> c -> d -> e -> r)
+  : interp_t =
+    fun psc cb us args ->
+      match args with
+      | [(a, _); (b, _); (c, _); (d, _); (e, _)] ->
+        let! r = f <$> try_unembed_simple a <*> try_unembed_simple b <*> try_unembed_simple c <*> try_unembed_simple d <*> try_unembed_simple e in
+        return (embed_simple psc.psc_range r)
+      | _ -> None
+
+let mk_nbe_interp5 #a #b #c #d #e #r
+  {| NBE.embedding a |}
+  {| NBE.embedding b |}
+  {| NBE.embedding c |}
+  {| NBE.embedding d |}
+  {| NBE.embedding e |}
+  {| NBE.embedding r |}
+  (f : a -> b -> c -> d -> e -> r)
+  : nbe_interp_t =
+    fun cbs us args ->
+      match args with
+      | [(a, _); (b, _); (c, _); (d, _); (e, _)] ->
+        let! r = f <$> NBE.unembed solve cbs a <*> NBE.unembed solve cbs b <*> NBE.unembed solve cbs c <*> NBE.unembed solve cbs d <*> NBE.unembed solve cbs e in
+        return (NBE.embed solve cbs r)
+      | _ ->
+        None
+
+let mk1 #a #r
+  (u_arity : int)
+  (name : Ident.lid)
+  {| EMB.embedding a |} {| NBE.embedding a |}
+  {| EMB.embedding r |} {| NBE.embedding r |}
+  (f : a -> r)
+  : primitive_step =
+  let interp : interp_t = mk_interp1 f in
+  let nbe_interp : nbe_interp_t = mk_nbe_interp1 f in
   as_primitive_step_nbecbs true (name, 1, u_arity, interp, nbe_interp)
 
 let mk2 #a #b #r
@@ -70,54 +200,8 @@ let mk2 #a #b #r
   {| EMB.embedding r |} {| NBE.embedding r |}
   (f : a -> b -> r)
   : primitive_step =
-  let interp : interp_t =
-    fun psc cb us args ->
-      match args with
-      | [(a, _); (b, _)] ->
-        let! r = f <$> try_unembed_simple a <*> try_unembed_simple b in
-        return (embed_simple psc.psc_range r)
-      | _ -> None
-  in
-  let nbe_interp : nbe_interp_t =
-    fun cbs us args ->
-      match args with
-      | [(a, _); (b, _)] ->
-        let! r = f <$> NBE.unembed solve cbs a <*> NBE.unembed solve cbs b in
-        return (NBE.embed solve cbs r)
-      | _ ->
-        None
-  in
-  as_primitive_step_nbecbs true (name, 2, u_arity, interp, nbe_interp)
-
-(* Duplication for op_Division / op_Modulus which can prevent reduction. The `f`
-already returns something in the option monad, so we add an extra join. *)
-let mk2' #a #b #r
-  (u_arity : int)
-  (name : Ident.lid)
-  {| EMB.embedding a |} {| NBE.embedding a |}
-  {| EMB.embedding b |} {| NBE.embedding b |}
-  {| EMB.embedding r |} {| NBE.embedding r |}
-  (f : a -> b -> option r)
-  : primitive_step =
-  let interp : interp_t =
-    fun psc cb us args ->
-      match args with
-      | [(a, _); (b, _)] ->
-        let! r = f <$> try_unembed_simple a <*> try_unembed_simple b in
-        let! r = r in
-        return (embed_simple psc.psc_range r)
-      | _ -> None
-  in
-  let nbe_interp : nbe_interp_t =
-    fun cbs us args ->
-      match args with
-      | [(a, _); (b, _)] ->
-        let! r = f <$> NBE.unembed solve cbs a <*> NBE.unembed solve cbs b in
-        let! r = r in
-        return (NBE.embed solve cbs r)
-      | _ ->
-        None
-  in
+  let interp : interp_t = mk_interp2 f in
+  let nbe_interp : nbe_interp_t = mk_nbe_interp2 f in
   as_primitive_step_nbecbs true (name, 2, u_arity, interp, nbe_interp)
 
 let mk3 #a #b #c #r
@@ -129,23 +213,8 @@ let mk3 #a #b #c #r
   {| EMB.embedding r |} {| NBE.embedding r |}
   (f : a -> b -> c -> r)
   : primitive_step =
-  let interp : interp_t =
-    fun psc cb us args ->
-      match args with
-      | [(a, _); (b, _); (c, _)] ->
-        let! r = f <$> try_unembed_simple a <*> try_unembed_simple b <*> try_unembed_simple c in
-        return (embed_simple psc.psc_range r)
-      | _ -> None
-  in
-  let nbe_interp : nbe_interp_t =
-    fun cbs us args ->
-      match args with
-      | [(a, _); (b, _); (c, _)] ->
-        let! r = f <$> NBE.unembed solve cbs a <*> NBE.unembed solve cbs b <*> NBE.unembed solve cbs c in
-        return (NBE.embed solve cbs r)
-      | _ ->
-        None
-  in
+  let interp : interp_t = mk_interp3 f in
+  let nbe_interp : nbe_interp_t = mk_nbe_interp3 f in
   as_primitive_step_nbecbs true (name, 3, u_arity, interp, nbe_interp)
 
 let mk4 #a #b #c #d #r
@@ -158,23 +227,8 @@ let mk4 #a #b #c #d #r
   {| EMB.embedding r |} {| NBE.embedding r |}
   (f : a -> b -> c -> d -> r)
   : primitive_step =
-  let interp : interp_t =
-    fun psc cb us args ->
-      match args with
-      | [(a, _); (b, _); (c, _); (d, _); (e, _)] ->
-        let! r = f <$> try_unembed_simple a <*> try_unembed_simple b <*> try_unembed_simple c <*> try_unembed_simple d in
-        return (embed_simple psc.psc_range r)
-      | _ -> None
-  in
-  let nbe_interp : nbe_interp_t =
-    fun cbs us args ->
-      match args with
-      | [(a, _); (b, _); (c, _); (d, _)] ->
-        let! r = f <$> NBE.unembed solve cbs a <*> NBE.unembed solve cbs b <*> NBE.unembed solve cbs c <*> NBE.unembed solve cbs d in
-        return (NBE.embed solve cbs r)
-      | _ ->
-        None
-  in
+  let interp : interp_t = mk_interp4 f in
+  let nbe_interp : nbe_interp_t = mk_nbe_interp4 f in
   as_primitive_step_nbecbs true (name, 4, u_arity, interp, nbe_interp)
 
 let mk5 #a #b #c #d #e #r
@@ -188,21 +242,67 @@ let mk5 #a #b #c #d #e #r
   {| EMB.embedding r |} {| NBE.embedding r |}
   (f : a -> b -> c -> d -> e -> r)
   : primitive_step =
+  let interp : interp_t = mk_interp5 f in
+  let nbe_interp : nbe_interp_t = mk_nbe_interp5 f in
+  as_primitive_step_nbecbs true (name, 5, u_arity, interp, nbe_interp)
+
+let mk2' #a #b #r #na #nb #nr
+  (u_arity : int)
+  (name : Ident.lid)
+  {| EMB.embedding a |} {| NBE.embedding na |}
+  {| EMB.embedding b |} {| NBE.embedding nb |}
+  {| EMB.embedding r |} {| NBE.embedding nr |}
+  (f : a -> b -> option r)
+  (nbe_f : na -> nb -> option nr)
+  : primitive_step =
   let interp : interp_t =
     fun psc cb us args ->
       match args with
-      | [(a, _); (b, _); (c, _); (d, _); (e, _)] ->
-        let! r = f <$> try_unembed_simple a <*> try_unembed_simple b <*> try_unembed_simple c <*> try_unembed_simple d <*> try_unembed_simple e in
+      | [(a, _); (b, _)] ->
+        let! r = f <$> try_unembed_simple a <*> try_unembed_simple b in
+        let! r = r in
         return (embed_simple psc.psc_range r)
       | _ -> None
   in
   let nbe_interp : nbe_interp_t =
     fun cbs us args ->
       match args with
-      | [(a, _); (b, _); (c, _); (d, _); (e, _)] ->
-        let! r = f <$> NBE.unembed solve cbs a <*> NBE.unembed solve cbs b <*> NBE.unembed solve cbs c <*> NBE.unembed solve cbs d <*> NBE.unembed solve cbs e in
+      | [(a, _); (b, _)] ->
+        let! r = nbe_f <$> NBE.unembed solve cbs a <*> NBE.unembed solve cbs b in
+        let! r = r in
         return (NBE.embed solve cbs r)
       | _ ->
         None
   in
-  as_primitive_step_nbecbs true (name, 5, u_arity, interp, nbe_interp)
+  as_primitive_step_nbecbs true (name, 2, u_arity, interp, nbe_interp)
+
+let mk3' #a #b #c #r #na #nb #nc #nr
+  (u_arity : int)
+  (name : Ident.lid)
+  {| EMB.embedding a |} {| NBE.embedding na |}
+  {| EMB.embedding b |} {| NBE.embedding nb |}
+  {| EMB.embedding c |} {| NBE.embedding nc |}
+  {| EMB.embedding r |} {| NBE.embedding nr |}
+  (f : a -> b -> c -> option r)
+  (nbe_f : na -> nb -> nc -> option nr)
+  : primitive_step =
+  let interp : interp_t =
+    fun psc cb us args ->
+      match args with
+      | [(a, _); (b, _); (c, _)] ->
+        let! r = f <$> try_unembed_simple a <*> try_unembed_simple b <*> try_unembed_simple c in
+        let! r = r in
+        return (embed_simple psc.psc_range r)
+      | _ -> None
+  in
+  let nbe_interp : nbe_interp_t =
+    fun cbs us args ->
+      match args with
+      | [(a, _); (b, _); (c, _)] ->
+        let! r = nbe_f <$> NBE.unembed solve cbs a <*> NBE.unembed solve cbs b <*> NBE.unembed solve cbs c in
+        let! r = r in
+        return (NBE.embed solve cbs r)
+      | _ ->
+        None
+  in
+  as_primitive_step_nbecbs true (name, 3, u_arity, interp, nbe_interp)
