src/typechecker/FStar.TypeChecker.Primops.Eq.fst
@@ -1,0 +1,46 @@
+module FStar.TypeChecker.Primops.Eq
+
+open FStar
+open FStar.Compiler
+open FStar.Compiler.Effect
+open FStar.Compiler.List
+open FStar.Syntax.Syntax
+open FStar.TypeChecker
+open FStar.Class.Monad
+open FStar.Class.Show
+
+module PC = FStar.Parser.Const
+module U  = FStar.Syntax.Util
+module EMB = FStar.Syntax.Embeddings
+module NBE = FStar.TypeChecker.NBETerm
+
+open FStar.TypeChecker.Primops.Base
+
+type abstract_term = | Abstract : t:term -> abstract_term
+instance _ : EMB.embedding abstract_term =
+  EMB.embed_as EMB.e_any (fun x -> Abstract x) (fun x -> match x with Abstract x -> x) None
+
+type abstract_nbe_term = | AbstractNBE : t:NBETerm.t -> abstract_nbe_term
+
+instance _ : NBE.embedding abstract_nbe_term =
+  NBE.embed_as NBE.e_any (fun x -> AbstractNBE x) (fun x -> match x with AbstractNBE x -> x) None
+
+let s_eq (_typ x y : abstract_term) : option bool =
+  match U.eq_tm x.t y.t with
+  | U.Equal -> Some true
+  | U.NotEqual -> Some false
+  | _ -> None
+
+let nbe_eq (_typ x y : abstract_nbe_term) : option bool =
+  match NBETerm.eq_t x.t y.t with
+  | U.Equal -> Some true
+  | U.NotEqual -> Some false
+  | _ -> None
+
+let push3 f g x y z = f (g x y z)
+let negopt3 = push3 (fmap #option not)
+
+let dec_eq_ops : list primitive_step = [
+  mk3' 0 PC.op_Eq     s_eq           nbe_eq;
+  mk3' 0 PC.op_notEq (negopt3 s_eq) (negopt3 nbe_eq);
+]
